src/monoidal_categories/util/data/bin_tree.lean
@@ -2,31 +2,31 @@ import .nonempty_list
 
 open util.data.nonempty_list
 
-namespace util.data.bin_tree
+namespace util.data.bin_tree'
 
 universes u v
 
-inductive bin_tree (α : Type u)
-| leaf : α → bin_tree
-| branch : bin_tree → bin_tree → bin_tree
+inductive bin_tree' (α : Type u)
+| leaf : α → bin_tree'
+| branch : bin_tree' → bin_tree' → bin_tree'
 
-namespace bin_tree
+namespace bin_tree'
 
 variables {α : Type u} {β : Type v}
 
-def map (f : α → β) : bin_tree α → bin_tree β
+def map (f : α → β) : bin_tree' α → bin_tree' β
 | (leaf x) := leaf (f x)
 | (branch l r) := branch (map l) (map r)
 
-def to_list : bin_tree α → nonempty_list α
+def to_list : bin_tree' α → nonempty_list α
 | (leaf x) := nonempty_list.singleton x
 | (branch l r) := to_list l ++  to_list r
 
-def size : bin_tree α → ℕ
+def size : bin_tree' α → ℕ
 | (leaf _) := 1
 | (branch l r) := size l + size r
 
-def from_list_lopsided : nonempty_list α → bin_tree α
+def from_list_lopsided : nonempty_list α → bin_tree' α
 | (nonempty_list.singleton x) := leaf x
 | (nonempty_list.cons x xs)   := branch (leaf x) (from_list_lopsided xs)
 
@@ -40,14 +40,14 @@ lemma from_list_lopsided_to_list : Π (l : nonempty_list α), to_list (from_list
     reflexivity
   end
 
-@[reducible] def lopsided (t : bin_tree α) : bin_tree α := from_list_lopsided t.to_list
+@[reducible] def lopsided (t : bin_tree' α) : bin_tree' α := from_list_lopsided t.to_list
 
-lemma lopsided_idempotent (t : bin_tree α) : t.lopsided.lopsided = t.lopsided :=
+lemma lopsided_idempotent (t : bin_tree' α) : t.lopsided.lopsided = t.lopsided :=
   begin
     unfold lopsided,
     rewrite from_list_lopsided_to_list (to_list t)
   end
 
-end bin_tree
+end bin_tree'
 
-end util.data.bin_tree
+end util.data.bin_tree'
