src/monoidal_categories/util/data/bin_tree/cong_clos.lean
@@ -2,8 +2,8 @@ import ..bin_tree
 import ..nonempty_list
 
 open util.data.nonempty_list
-open util.data.bin_tree
-open util.data.bin_tree.bin_tree
+open util.data.bin_tree'
+open util.data.bin_tree'.bin_tree'
 
 universes u v
 
@@ -12,7 +12,7 @@ variable {α : Type u}
 -- https://ncatlab.org/nlab/show/Mac+Lane%27s+proof+of+the+coherence+theorem+for+monoidal+categories
 
 -- TODO(tim): do we really need two definitions of the congruence closure or can we just delete this one?
-inductive cong_clos' (R : bin_tree α → bin_tree α → Type u) : bin_tree α → bin_tree α → Type u
+inductive cong_clos' (R : bin_tree' α → bin_tree' α → Type u) : bin_tree' α → bin_tree' α → Type u
 | lift : Π s t, R s t → cong_clos' s t
 | refl : Π t, cong_clos' t t
 | trans : Π r s t, cong_clos' r s → cong_clos' s t → cong_clos' r t
@@ -20,7 +20,7 @@ inductive cong_clos' (R : bin_tree α → bin_tree α → Type u) : bin_tree α 
 
 namespace cong_clos'
 
-variable {R : bin_tree α → bin_tree α → Type u}
+variable {R : bin_tree' α → bin_tree' α → Type u}
 
 def sym (R_sym : Π s t, R s t → R t s)
     : Π {s t}, cong_clos' R s t → cong_clos' R t s
@@ -29,7 +29,7 @@ def sym (R_sym : Π s t, R s t → R t s)
 | ._ ._ (trans _ _ _ p q)  := trans _ _ _ (sym q) (sym p)
 | ._ ._ (cong _ _ _ _ l r) := cong _ _ _ _ (sym l) (sym r)
 
-def transport {S : bin_tree α → bin_tree α → Type u} (f : Π s t, R s t → S s t)
+def transport {S : bin_tree' α → bin_tree' α → Type u} (f : Π s t, R s t → S s t)
     : Π {s t}, cong_clos' R s t → cong_clos' S s t
 | ._ ._ (lift _ _ p)       := lift _ _ (f _ _ p)
 | ._ ._ (refl ._ t)        := refl S t
@@ -43,21 +43,21 @@ lemma respects_to_list (R_to_list : Π s t, R s t → s.to_list = t.to_list)
 | ._ ._ (trans _ _ _ p q)      := eq.trans (respects_to_list p) (respects_to_list q)
 | ._ ._ (cong l₁ r₁ l₂ r₂ l r) :=
     begin
-      unfold bin_tree.to_list,
+      unfold bin_tree'.to_list,
       rewrite (respects_to_list l),
       rewrite (respects_to_list r)
     end
 
 end cong_clos'
 
-inductive cong_clos_step (R : bin_tree α → bin_tree α → Type u) : bin_tree α → bin_tree α → Type u
+inductive cong_clos_step (R : bin_tree' α → bin_tree' α → Type u) : bin_tree' α → bin_tree' α → Type u
 | lift  : Π s t, R s t → cong_clos_step s t
 | left  : Π l₁ l₂ r, cong_clos_step l₁ l₂ → cong_clos_step (branch l₁ r) (branch l₂ r)
 | right : Π l r₁ r₂, cong_clos_step r₁ r₂ → cong_clos_step (branch l r₁) (branch l r₂)
 
 namespace cong_clos_step
 
-variable {R : bin_tree α → bin_tree α → Type u}
+variable {R : bin_tree' α → bin_tree' α → Type u}
 
 -- the equation compiler somehow can't handle the next definitions ~> turn it off
 -- TODO(tim): report bug
@@ -69,7 +69,7 @@ def sym (R_sym : Π s t, R s t → R t s)
 | ._ ._ (left _ _ _ l)  := left _ _ _ (sym l)
 | ._ ._ (right _ _ _ r) := right _ _ _ (sym r)
 
-def transport {S : bin_tree α → bin_tree α → Type u} (f : Π s t, R s t → S s t)
+def transport {S : bin_tree' α → bin_tree' α → Type u} (f : Π s t, R s t → S s t)
     : Π {s t}, cong_clos_step R s t → cong_clos_step S s t
 | ._ ._ (lift _ _ p)    := lift _ _ (f _ _ p)
 | ._ ._ (left _ _ _ l)  := left _ _ _ (transport l)
@@ -78,8 +78,8 @@ def transport {S : bin_tree α → bin_tree α → Type u} (f : Π s t, R s t �
 lemma respects_to_list (R_to_list : Π s t, R s t → s.to_list = t.to_list)
     : Π {s t}, cong_clos_step R s t → s.to_list = t.to_list
 | ._ ._ (lift _ _ p)    := R_to_list _ _ p
-| ._ ._ (left _ _ _ l)  := by unfold bin_tree.to_list; rewrite (respects_to_list l)
-| ._ ._ (right _ _ _ r) := by unfold bin_tree.to_list; rewrite (respects_to_list r)
+| ._ ._ (left _ _ _ l)  := by unfold bin_tree'.to_list; rewrite (respects_to_list l)
+| ._ ._ (right _ _ _ r) := by unfold bin_tree'.to_list; rewrite (respects_to_list r)
 
 lemma respects_lopsided
     (R_to_list : Π s t, R s t → s.to_list = t.to_list)
@@ -92,39 +92,39 @@ set_option eqn_compiler.lemmas true
 end cong_clos_step
 
 -- smallest reflexive, transitive, congruent (but not necessarily symmetric) relation that includes R
-inductive cong_clos (R : bin_tree α → bin_tree α → Type u) : bin_tree α → bin_tree α → Type u
+inductive cong_clos (R : bin_tree' α → bin_tree' α → Type u) : bin_tree' α → bin_tree' α → Type u
 | refl : Π t, cong_clos t t
 | step : Π r s t, cong_clos_step R r s → cong_clos s t → cong_clos r t
 
 namespace cong_clos
 
-variable {R : bin_tree α → bin_tree α → Type u}
+variable {R : bin_tree' α → bin_tree' α → Type u}
 
 open cong_clos_step
 
-def lift {s t : bin_tree α} (p : R s t) : cong_clos R s t :=
+def lift {s t : bin_tree' α} (p : R s t) : cong_clos R s t :=
   step _ _ _ (cong_clos_step.lift _ _ p) (refl R _)
 
-def trans : Π {r s t : bin_tree α}, cong_clos R r s → cong_clos R s t → cong_clos R r t
+def trans : Π {r s t : bin_tree' α}, cong_clos R r s → cong_clos R s t → cong_clos R r t
 | ._ ._ _ (refl ._ t)       qs := qs
 | ._ ._ _ (step _ _ _ p ps) qs := step _ _ _ p (trans ps qs)
 
-lemma trans_refl_right : Π {s t : bin_tree α} (p : cong_clos R s t), trans p (refl R t) = p
+lemma trans_refl_right : Π {s t : bin_tree' α} (p : cong_clos R s t), trans p (refl R t) = p
 | ._ ._ (refl ._ t)       := by reflexivity
 | ._ ._ (step _ _ _ p ps) := by unfold trans; rewrite (trans_refl_right ps)
 
-def inject_left (r : bin_tree α) : Π {l₁ l₂ : bin_tree α}, cong_clos R l₁ l₂ → cong_clos R (branch l₁ r) (branch l₂ r)
+def inject_left (r : bin_tree' α) : Π {l₁ l₂ : bin_tree' α}, cong_clos R l₁ l₂ → cong_clos R (branch l₁ r) (branch l₂ r)
 | ._ ._ (refl ._ t)       := refl R _
 | ._ ._ (step _ _ _ p ps) := step _ _ _ (left _ _ _ p) (inject_left ps)
 
-def inject_right (l : bin_tree α) : Π {r₁ r₂ : bin_tree α}, cong_clos R r₁ r₂ → cong_clos R (branch l r₁) (branch l r₂)
+def inject_right (l : bin_tree' α) : Π {r₁ r₂ : bin_tree' α}, cong_clos R r₁ r₂ → cong_clos R (branch l r₁) (branch l r₂)
 | ._ ._ (refl ._ _)       := refl R _
 | ._ ._ (step _ _ _ p ps) := step _ _ _ (right _ _ _ p) (inject_right ps)
 
-def cong {l₁ l₂ r₁ r₂ : bin_tree α} (l : cong_clos R l₁ l₂) (r : cong_clos R r₁ r₂) : cong_clos R (branch l₁ r₁) (branch l₂ r₂) :=
+def cong {l₁ l₂ r₁ r₂ : bin_tree' α} (l : cong_clos R l₁ l₂) (r : cong_clos R r₁ r₂) : cong_clos R (branch l₁ r₁) (branch l₂ r₂) :=
   trans (inject_left _ l) (inject_right _ r)
 
-def convert : Π (s t : bin_tree α), cong_clos' R s t → cong_clos R s t
+def convert : Π (s t : bin_tree' α), cong_clos' R s t → cong_clos R s t
 | ._ ._ (cong_clos'.refl ._ _)        := refl R _
 | ._ ._ (cong_clos'.lift _ _ p)       := lift p
 | ._ ._ (cong_clos'.trans _ _ _ p q)  := trans (convert _ _ p) (convert _ _ q)
@@ -138,7 +138,7 @@ def sym_helper (R_sym : Π s t, R s t → R t s)
 def sym (R_sym : Π s t, R s t → R t s) {s t} (ps : cong_clos R s t) : cong_clos R t s :=
   sym_helper R_sym ps (refl R _)
 
-def transport {S : bin_tree α → bin_tree α → Type u} (f : Π s t, R s t → S s t)
+def transport {S : bin_tree' α → bin_tree' α → Type u} (f : Π s t, R s t → S s t)
     : Π {s t}, cong_clos R s t → cong_clos S s t
 | ._ ._ (refl ._ t)       := refl S t
 | ._ ._ (step _ _ _ p ps) := step _ _ _ (cong_clos_step.transport f p) (transport ps)
